open exhaustive

Core/Infer/Global.lean
@@ -55,93 +55,6 @@ def GlobalEnv.wf_globals : GlobalEnv -> Option Unit
   if (lookup x G).isNone
   then return () else none
 
--- def OpenExhaustive (G : List Global) : Prop :=
---   ∀ {x na nb} {τ : Subst Ty} {As Ks : Vec _ na} {Ts Ts' : Vec _ nb} {Δ R q},
---   lookup x G = some (.openm x ⟨na, Ks, nb, Ts, R⟩) ->
---   (∀ (i : Fin na), G&Δ ⊢ As[i] : Ks[i]) ->
---   Sequ.append_vec (Vec.map su As) +0 = τ ->
---   Vec.map (·[τ]) Ts = Ts' ->
---   Query G .opn q Ts' ->
---   ∃ (i : Nat), ∃ b p, G[i]? = some (.inst x p b) ∧ Query.Match q p
-
-def List.enumerate (l : List α) : List (Nat × α) :=
-  let t := List.foldl (λ (i, acc) x => (i + 1, acc ++ [(i, x)])) (0, .nil) l
-  t.snd
-
-theorem List.enumerate_length {ls : List α} {ls' : List (Nat × α)}:
-  List.enumerate ls = ls' ->
-  ls'.length = ls.length := by sorry
-
-theorem List.enumerate_indexing {ls : List α} {ls' : List (Nat × α)}:
-  ∀ (h : i < ls.length),
-  (h2 : List.enumerate ls = ls') ->
-  ls'[i]'(by rw[List.enumerate_length (ls := ls) (ls' := ls')]; apply h; apply h2) = (i, ls[i])
-:= by
-  intro h1 h2
-  unfold List.enumerate at h2
-  simp at h2;
-
-  sorry
-
-def List.map_prov :
-  List.map f ls = vs ->
-  ∀ v ∈ vs, ∃ l ∈ ls, f l = v := by
-intro h v v_in_vs
-fun_induction List.map generalizing vs
-subst h; simp at v_in_vs
-case _ hd tl ih =>
-  cases v_in_vs
-  case _ => exists hd; simp; simp at h; apply h.1
-  case _ b as v_in_vs =>
-    simp at h;
-    replace ih := ih h.2 v_in_vs
-    rcases ih with ⟨l, ih1, ih2⟩
-    exists l; apply And.intro;
-    simp; apply Or.inr ih1
-    apply ih2
-
-def List.filter_prov :
-  List.filter f ls = vs ->
-  ∀ v ∈ vs, ∃ l ∈ ls, f l = true := by
-intro h v v_in_vs
-fun_induction List.filter f ls generalizing vs
-subst h; simp at v_in_vs
-case _ hd tl p ih =>
-  cases v_in_vs
-  · simp at h; rcases h with ⟨e, h⟩;
-    subst e; subst h; exists hd; simp; apply p
-  case _ v_in_vs =>
-    simp at h; rcases h with ⟨e, h⟩;
-    subst e; replace ih := ih h v_in_vs;
-    rcases ih with ⟨l, ih1, ih2⟩
-    exists l; simp
-    apply And.intro (Or.inr ih1) ih2
-case _ ih =>
-  replace ih := ih h v_in_vs
-  rcases ih with ⟨l, ih1, ih2⟩
-  exists l; simp;
-  apply And.intro (Or.inr ih1) ih2
-
-def List.filter_then_map_prov :
-  List.map f (List.filter p ls) = vs ->
-  ∀ v ∈ vs, ∃ l ∈ ls, p l = true ∧ f l = v := by
-intro h v v_in_vs
-
-sorry
--- generalize zdef : List.filter p ls = zs at *
--- intro h v v_in_vs
-
--- have lem2 := List.map_prov h v v_in_vs
--- rcases lem2 with ⟨z, z_in_zs, zh⟩
--- have lem1 := List.filter_prov zdef z z_in_zs
--- rcases lem1 with ⟨l, l_in_ls, lh⟩
--- subst zdef;
--- have lem : z ∈ List.filter p ls -> z ∈ ls := by
-
---   sorry
--- exists l; exists l_in_ls; apply And.intro lh
-
--- sorry
 
 
 def mk_open_pattern (x : String) (nc : Nat) :
@@ -152,39 +65,8 @@ def mk_open_pattern (x : String) (nc : Nat) :
            else none
 | _ => none
 
-def mk_open_pattern_attach {G : GlobalEnv} (x : String) (nc : Nat) :
-  {x : Global // x ∈ G} -> Option ({g : Global // g ∈ G})
-| ⟨.inst (m := m) y p t, prop ⟩=>
-           if h : y == x && m == nc
-           then let p' : Pattern nc := (p |> cast (by simp at h; rw[h.2]))
-                let prop' : Global.inst y p' t ∈ G := (prop |> cast (by simp at h; grind))
-                return ⟨.inst (m := m) y p t, prop⟩
-           else none
-| _ => none
-
-
-
-def mk_open_patterns (G : GlobalEnv) (x : String) (nc : Nat) :
-    List (Pattern nc) :=
-  match G with
-  | .nil  => .nil
-  | .cons g gs =>
-    let ps := mk_open_patterns gs x nc
-    match mk_open_pattern x nc g with
-    | some p => p :: ps
-    | none => ps
-
-def mk_open_patterns_attach_aux (x : String) (nc : Nat) {G : GlobalEnv} : List {x : Global // x ∈ G} ->
-    List ({g : Global // g ∈ G})
-  | .nil => .nil
-  | .cons g gs =>
-    let ps := mk_open_patterns_attach_aux x nc gs
-    match mk_open_pattern_attach x nc g with
-    | some p => p :: ps
-    | none => ps
-
-def mk_open_patterns_attach (x : String) (nc : Nat) (G : GlobalEnv)
-  := mk_open_patterns_attach_aux x nc (G := G) G.attach
+def mk_open_patterns (G : GlobalEnv) (x : String) (nc : Nat) : List (Pattern nc) :=
+  G.filterMap (λ g => mk_open_pattern x nc g)
 
 
 def GlobalEnv.check_insts (G : GlobalEnv) : Global -> Option Unit
